refactor compileCorrectnessScript.sml
split off compileLabelsTheory

compiler/correctness/compileCorrectnessScript.sml
@@ -1,5 +1,5 @@
 open HolKernel bossLib boolLib boolSimps SatisfySimps listTheory rich_listTheory pairTheory pred_setTheory finite_mapTheory alistTheory relationTheory arithmeticTheory lcsymtacs quantHeuristicsLib quantHeuristicsLibAbbrev
-open MiniMLTerminationTheory miniMLExtraTheory miscTheory compileTerminationTheory intLangTheory bytecodeTerminationTheory evaluateEquationsTheory expToCexpTheory pmatchTheory labelClosuresTheory bytecodeEvalTheory
+open MiniMLTerminationTheory miniMLExtraTheory miscTheory compileTerminationTheory intLangTheory bytecodeTerminationTheory evaluateEquationsTheory expToCexpTheory pmatchTheory labelClosuresTheory bytecodeEvalTheory bytecodeExtraTheory
 val _ = intLib.deprecate_int()
 val _ = new_theory "compileCorrectness"
 
@@ -101,7 +101,7 @@ val Cexp_pred_calculate_ldefs = store_thm("Cexp_pred_calculate_ldefs",
   first_x_assum (match_mp_tac o MP_CANON) >>
   fs[EVERY_MEM])
 
-val _ = overload_on("next_addr", ``λil ls. SUM (MAP (SUC o il) (FILTER ($~ o is_Label) ls))``)
+val _ = Parse.overload_on("next_addr", ``λil ls. SUM (MAP (SUC o il) (FILTER ($~ o is_Label) ls))``)
 
 val bc_finish_def = Define`
   bc_finish s1 s2 = bc_next^* s1 s2 ∧ (s2.pc = next_addr s2.inst_length s2.code)`
@@ -355,11 +355,10 @@ val v_to_Cv_ov = store_thm("v_to_Cv_ov",
   srw_tac[ETA_ss][fmap_linv_FAPPLY])
 
 (* TODO: move *)
-val bc_find_loc_aux_def = BytecodeTheory.bc_find_loc_aux_def
 val prim2_to_bc_def = CompileTheory.prim2_to_bc_def
 val _ = export_rewrites["Compile.prim2_to_bc_def"]
 
-val _ = overload_on("mk_pp", ``λc bs.
+val _ = Parse.overload_on("mk_pp", ``λc bs.
   (c
   ,combin$C (bc_find_loc_aux bs.code bs.inst_length) 0
   ,bs.refs
@@ -376,27 +375,6 @@ val env_rs_def = Define`
   env_rs env bs rs =
     let Cenv = alist_to_fmap (env_to_Cenv (cmap rs.contab) env) in
     ∃c. Cenv_bs c Cenv rs.renv rs.rsz bs`
-
-val el_of_addr_def = Define`
-  (el_of_addr il n [] = NONE) ∧
-  (el_of_addr il n (x::xs) =
-   if is_Label x then OPTION_BIND (el_of_addr il n xs) (λm. SOME (m + 1)) else
-     if n = 0 then SOME (0:num) else
-       if n < il x + 1 then NONE else
-         OPTION_BIND (el_of_addr il (n - (il x + 1)) xs) (λm. SOME (m + 1)))`
-val _ = export_rewrites["el_of_addr_def"]
-
-val el_of_addr_LESS_LENGTH = store_thm("el_of_addr_LESS_LENGTH",
-  ``∀il ls n m. (el_of_addr il n ls = SOME m) ⇒ m < LENGTH ls``,
-  gen_tac >> Induct >> srw_tac[ARITH_ss][] >>
-  res_tac >> fsrw_tac[ARITH_ss][])
-
-val bc_fetch_aux_el_of_addr = store_thm("bc_fetch_aux_el_of_addr",
-  ``∀c il pc. bc_fetch_aux c il pc = OPTION_BIND (el_of_addr il pc c) (λn. SOME (EL n c))``,
-  Induct >> rw[] >>
-  Q.PAT_ABBREV_TAC`opt = el_of_addr il pcX c` >>
-  Cases_on `opt` >> fs[] >>
-  rw[GSYM arithmeticTheory.ADD1])
 
 val addr_of_el_def = Define`
   (addr_of_el il n [] = NONE) ∧
@@ -416,153 +394,6 @@ val bc_fetch_aux_not_label = store_thm("bc_fetch_aux_not_label",
   ``∀c il pc i. (bc_fetch_aux c il pc = SOME i) ⇒ ¬is_Label i``,
   Induct >> rw[] >> fs[] >> PROVE_TAC[])
 
-val dest_Label_def = Define`(dest_Label (Label n) = n)`
-val _ = export_rewrites["dest_Label_def"]
-
-val calculate_labels_thm = store_thm("calculate_labels_thm",
-  ``∀il m n bc lbc m' n' bc'.
-      (calculate_labels il m n bc lbc = (m',n',bc')) ∧ ALL_DISTINCT (FILTER is_Label lbc) ⇒
-      (bc' = (REVERSE (FILTER ($~ o is_Label) lbc) ++ bc)) ∧
-      (let ls = MAP dest_Label (FILTER is_Label lbc) in
-        (m' = m |++ ZIP (ls, MAP (THE o combin$C (bc_find_loc_aux lbc il) n) ls))) ∧
-      (n' = n + SUM (MAP (SUC o il) (FILTER ($~ o is_Label) lbc)))``,
-  ho_match_mp_tac calculate_labels_ind >>
-  strip_tac >- (
-    rw[calculate_labels_def,LET_THM,FUPDATE_LIST_THM] ) >>
-  strip_tac >- (
-    rpt gen_tac >> strip_tac >>
-    simp_tac(std_ss)[Once calculate_labels_def] >>
-    rpt gen_tac >> strip_tac >>
-    `ALL_DISTINCT (FILTER is_Label lbc)` by (
-      pop_assum mp_tac >>
-      rpt (pop_assum kall_tac) >>
-      rw[] ) >>
-    res_tac >>
-    full_simp_tac(std_ss)[LET_THM] >>
-    rpt BasicProvers.VAR_EQ_TAC >>
-    pop_assum kall_tac >> pop_assum mp_tac >>
-    rpt (pop_assum kall_tac) >>
-    rw[FUPDATE_LIST_THM,bc_find_loc_aux_def] >>
-    AP_TERM_TAC >> AP_TERM_TAC >> AP_TERM_TAC >>
-    rw[MAP_EQ_f,MEM_MAP,MEM_FILTER] >>
-    AP_TERM_TAC >>
-    rw[bc_find_loc_aux_def] >>
-    fs[MEM_FILTER] >>
-    Cases_on `y` >> fs[]) >>
-  REPEAT (
-    strip_tac >- (
-      rpt gen_tac >> strip_tac >>
-      simp_tac(std_ss)[Once calculate_labels_def] >>
-      rpt gen_tac >> strip_tac >>
-      `ALL_DISTINCT (FILTER is_Label lbc)` by (
-        pop_assum mp_tac >>
-        rpt (pop_assum kall_tac) >>
-        rw[] ) >>
-      res_tac >>
-      full_simp_tac(std_ss)[LET_THM] >>
-      rpt BasicProvers.VAR_EQ_TAC >>
-      rpt (pop_assum kall_tac) >>
-      srw_tac[ARITH_ss][] >>
-      AP_TERM_TAC >> AP_TERM_TAC >> AP_TERM_TAC >>
-      rw[MAP_EQ_f,MEM_MAP,MEM_FILTER] >>
-      AP_TERM_TAC >>
-      rw[bc_find_loc_aux_def] )))
-
-val replace_lab_def = Define`
-  (replace_lab m (Jump (Lab l)) = Jump (Addr (FAPPLY m l))) ∧
-  (replace_lab m (JumpIf (Lab l)) = JumpIf (Addr (m ' l))) ∧
-  (replace_lab m (Call (Lab l)) = Call (Addr (m ' l))) ∧
-  (replace_lab m (PushPtr (Lab l)) = PushPtr (Addr (m ' l))) ∧
-  (replace_lab m i = i)`
-val _ = export_rewrites["replace_lab_def"]
-
-val replace_labels_thm = store_thm("replace_labels_thm",
-  ``∀m a ls. (replace_labels m a ls = (REVERSE (MAP (replace_lab m) ls)) ++ a)``,
-  ho_match_mp_tac replace_labels_ind >> rw[replace_labels_def])
-
-val bc_fetch_aux_MAP = store_thm("bc_fetch_aux_MAP",
-  ``!il f. (∀x. il (f x) = il x) ∧ (∀x. is_Label (f x) = is_Label x) ⇒
-      ∀ls n. (bc_fetch_aux (MAP f ls) il n = OPTION_MAP f (bc_fetch_aux ls il n))``,
-  ntac 2 gen_tac >> strip_tac >>
-  Induct >> rw[bc_fetch_aux_def])
-
-val bc_fetch_MAP = store_thm("bc_fetch_MAP",
-  ``∀f s. (∀x. s.inst_length (f x) = s.inst_length x) ∧ (∀x. is_Label (f x) = is_Label x) ⇒
-    (bc_fetch (s with <| code := MAP f s.code |>) = OPTION_MAP f (bc_fetch s))``,
-  rw[bc_fetch_def,bc_fetch_aux_MAP])
-
-val is_Label_replace_lab = store_thm("is_Label_replace_lab",
-  ``∀x. is_Label (replace_lab m x) = is_Label x``,
-  Cases >> rw[] >> Cases_on `l` >> rw[])
-val _ = export_rewrites["is_Label_replace_lab"]
-
-val good_il_def = Define`
-  good_il il =
-  (∀x. il (Jump x) = il (Jump ARB)) ∧
-  (∀x. il (JumpIf x) = il (JumpIf ARB)) ∧
-  (∀x. il (Call x) = il (Call ARB)) ∧
-  (∀x. il (PushPtr x) = il (PushPtr ARB))`
-
-val il_replace_lab = store_thm("il_replace_lab",
-  ``good_il il ⇒ ∀m x. (il (replace_lab m x) = il x)``,
-  rw[good_il_def] >>
-  Cases_on `x` >> rw[] >>
-  Cases_on `l` >> rw[])
-
-val bc_fetch_with_stack = store_thm("bc_fetch_with_stack",
-  ``bc_fetch (s with stack := st) = bc_fetch s``,
-  rw[bc_fetch_def])
-
-val bump_pc_with_stack = store_thm("bump_pc_with_stack",
-  ``bump_pc (s with stack := st) = (bump_pc s) with stack := st``,
-  rw[bump_pc_def,bc_fetch_with_stack] >>
-  BasicProvers.EVERY_CASE_TAC)
-
-val tac = (
-    rw[LET_THM] >>
-    match_mp_tac bc_eval1_SOME >>
-    Q.PAT_ABBREV_TAC`f = replace_lab X` >>
-    qspecl_then[`f`,`s1`] mp_tac bc_fetch_MAP >>
-    qunabbrev_tac`f` >> rw[il_replace_lab] >>
-    rw[bc_eval1_def] >>
-    fs[bc_eval_stack_thm] >>
-    fs[bump_pc_def] )
-
-val tac2 = (
-    rw[LET_THM] >>
-    match_mp_tac bc_eval1_SOME >>
-    Q.PAT_ABBREV_TAC`f = replace_lab X` >>
-    qspecl_then[`f`,`s1`] mp_tac bc_fetch_MAP >>
-    qunabbrev_tac`f` >>
-    Cases_on `l` >> rw[il_replace_lab] >>
-    srw_tac[DNF_ss][bc_eval1_def,LET_THM] >>
-    fs[bc_eval_stack_thm,bc_find_loc_def] >>
-    fs[FLOOKUP_DEF] >>
-    rw[bump_pc_with_stack] >>
-    rw[bump_pc_def] >>
-    fs[good_il_def] >>
-    metis_tac[optionTheory.SOME_11,optionTheory.NOT_SOME_NONE])
-
-val bc_next_MAP_replace_lab = store_thm("bc_next_MAP_replace_lab",
-  ``∀s1 s2. bc_next s1 s2 ⇒
-      ∀m. good_il s1.inst_length ∧
-      (∀l. FLOOKUP m l = bc_find_loc s1 (Lab l)) ⇒
-    let c = MAP (replace_lab m) s1.code in
-    bc_next (s1 with <| code := c |>) (s2 with <| code := c |>)``,
-  ho_match_mp_tac bc_next_ind >>
-  strip_tac >- tac >>
-  strip_tac >- tac2 >>
-  strip_tac >- tac2 >>
-  strip_tac >- tac2 >>
-  strip_tac >- tac >>
-  strip_tac >- tac >>
-  strip_tac >- tac2 >>
-  strip_tac >- tac >>
-  strip_tac >- tac >>
-  strip_tac >- tac >>
-  strip_tac >- tac >>
-  strip_tac >- tac )
-
 val labels_only_def = Define`
   (labels_only (Jump (Addr _)) = F) ∧
   (labels_only (JumpIf (Addr _)) = F) ∧
@@ -570,132 +401,6 @@ val labels_only_def = Define`
   (labels_only (PushPtr (Addr _)) = F) ∧
   (labels_only _ = T)`
 val _ = export_rewrites["labels_only_def"]
-
-val addrs_only_def = Define`
-  (addrs_only (Jump (Lab _)) = F) ∧
-  (addrs_only (JumpIf (Lab _)) = F) ∧
-  (addrs_only (Call (Lab _)) = F) ∧
-  (addrs_only (PushPtr (Lab _)) = F) ∧
-  (addrs_only _ = T)`
-val _ = export_rewrites["addrs_only_def"]
-
-val bc_fetch_aux_FILTER_labels = store_thm("bc_fetch_aux_FILTER_labels",
-  ``∀il ls n. bc_fetch_aux (FILTER ($~ o is_Label) ls) il n = bc_fetch_aux ls il n``,
-  gen_tac >> Induct >> rw[])
-val _ = export_rewrites["bc_fetch_aux_FILTER_labels"]
-
-val bc_fetch_FILTER_labels = store_thm("bc_fetch_FILTER_labels",
-  ``bc_fetch (s with code := FILTER ($~ o is_Label) s.code) = bc_fetch s``,
-  rw[bc_fetch_def])
-val _ = export_rewrites["bc_fetch_FILTER_labels"]
-
-val bc_fetch_MEM = store_thm("bc_fetch_MEM",
-  ``(bc_fetch s1 = SOME i) ⇒ (MEM i s1.code)``,
-  rw[bc_fetch_def] >>
-  fs[bc_fetch_aux_el_of_addr] >>
-  rw[MEM_EL] >>
-  imp_res_tac el_of_addr_LESS_LENGTH >>
-  metis_tac[])
-
-val bc_next_FILTER_labels = store_thm("bc_next_FILTER",
-  ``∀s1 s2. bc_next s1 s2 ⇒ EVERY addrs_only s1.code ⇒
-      let c = FILTER ($~ o is_Label) s1.code in
-      bc_next (s1 with <| code := c |>) (s2 with <| code := c |>)``,
-  ho_match_mp_tac bc_next_ind >>
-  rw[LET_THM] >>
-  rw[bc_eval1_thm] >>
-  srw_tac[DNF_ss][bc_eval1_def,LET_THM] >>
-  fs[bc_eval_stack_thm] >>
-  rw[bump_pc_def] >>
-  imp_res_tac bc_fetch_MEM >>
-  fs[EVERY_MEM] >>
-  res_tac >>
-  Cases_on `l` >> fs[bc_find_loc_def] >>
-  rw[bc_fetch_with_stack])
-
-val addrs_only_replace_lab = store_thm("addrs_only_replace_lab",
-  ``addrs_only (replace_lab m x)``,
-  Cases_on `x` >> rw[] >> Cases_on `l` >> rw[])
-val _ = export_rewrites["addrs_only_replace_lab"]
-
-val bc_find_loc_aux_NONE = store_thm("bc_find_loc_aux_NONE",
-  ``∀il l ls n. (bc_find_loc_aux ls il l n = NONE) ⇒ ¬MEM (Label l) ls``,
-  ntac 2 gen_tac >>
-  Induct >> rw[bc_find_loc_aux_def] >>
-  res_tac >> fs[])
-
-val bc_find_loc_aux_MEM = store_thm("bc_find_loc_aux_MEM",
-  ``∀il l ls n. (bc_find_loc_aux ls il l n ≠ NONE) ⇒ MEM (Label l) ls``,
-  ntac 2 gen_tac >>
-  Induct >> rw[bc_find_loc_aux_def] >>
-  res_tac)
-
-(* TODO: move *)
-val ALL_DISTINCT_MAP_INJ = store_thm("ALL_DISTINCT_MAP_INJ",
-  ``!ls f. (!x y. MEM x ls /\ MEM y ls /\ (f x = f y) ==> (x = y)) /\ ALL_DISTINCT ls  ==> ALL_DISTINCT (MAP f ls)``,
-  Induct THEN SRW_TAC[][MEM_MAP] THEN PROVE_TAC[])
-
-val bc_next_compile_labels = store_thm("bc_next_compile_labels",
-  ``∀s1 s2. bc_next s1 s2 ⇒
-      (good_il s1.inst_length ∧
-       ALL_DISTINCT (FILTER is_Label s1.code)) ⇒
-      let c = compile_labels s1.inst_length s1.code in
-      bc_next (s1 with <| code := c |>) (s2 with <| code := c |>)``,
-  rw[compile_labels_def,replace_labels_thm] >>
-  imp_res_tac calculate_labels_thm >>
-  rpt BasicProvers.VAR_EQ_TAC >>
-  qunabbrev_tac`c` >>
-  rw[MAP_REVERSE] >>
-  `∀x. ($~ o is_Label) (replace_lab m x) = ($~ o is_Label) x` by rw[] >>
-  rw[MAP_FILTER] >>
-  qmatch_abbrev_tac `bc_next (s1 with code := FILTER P ls) (s2 with code := FILTER P ls)` >>
-  `EVERY addrs_only ls` by (
-    qunabbrev_tac`ls` >>
-    rw[EVERY_MAP] ) >>
-  `bc_next (s1 with code := ls) (s2 with code := ls)` by (
-    qunabbrev_tac`ls` >>
-    match_mp_tac (MP_CANON(SIMP_RULE(srw_ss())[LET_THM]bc_next_MAP_replace_lab)) >>
-    rw[bc_find_loc_def] >>
-    fs[LET_THM] >>
-    qmatch_abbrev_tac `FLOOKUP (fm |++ ls) l = X` >>
-    Cases_on `X` >- (
-      `ALOOKUP (REVERSE ls) l = NONE` by (
-        qunabbrev_tac`ls` >>
-        rw[ALOOKUP_FAILS,ZIP_MAP] >>
-        rw[MAP_MAP_o,combinTheory.o_DEF] >>
-        `¬MEM (Label l) s1.code` by metis_tac[bc_find_loc_aux_NONE] >>
-        `¬MEM (Label l) (FILTER is_Label s1.code)` by rw[MEM_FILTER] >>
-        rw[MEM_MAP] >>
-        Cases_on `x` >> rw[MEM_FILTER] >>
-        PROVE_TAC[] ) >>
-      imp_res_tac FLOOKUP_FUPDATE_LIST_ALOOKUP_NONE >>
-      fs[Abbr`fm`] ) >>
-    `ALOOKUP (REVERSE ls) l = SOME x` by (
-      match_mp_tac ALOOKUP_ALL_DISTINCT_MEM >>
-      qunabbrev_tac`ls` >>
-      rw[REVERSE_ZIP,MAP_ZIP,ALL_DISTINCT_REVERSE] >- (
-        match_mp_tac ALL_DISTINCT_MAP_INJ >> fs[] >>
-        qx_gen_tac `a` >> qx_gen_tac `b` >>
-        Cases_on `a` >> Cases_on `b` >> rw[MEM_FILTER] ) >>
-      `MEM (Label l) s1.code` by
-        metis_tac[bc_find_loc_aux_MEM,optionTheory.NOT_SOME_NONE] >>
-      `MEM (Label l) (FILTER is_Label s1.code)` by rw[MEM_FILTER] >>
-      pop_assum (strip_assume_tac o SIMP_RULE (srw_ss()) [MEM_EL]) >>
-      rw[MEM_ZIP] >>
-      qexists_tac `n` >>
-      pop_assum (assume_tac o SYM) >>
-      rw[EL_MAP] ) >>
-    imp_res_tac FLOOKUP_FUPDATE_LIST_ALOOKUP_SOME >>
-    fs[] ) >>
-  qunabbrev_tac`P` >>
-  `ls = (s1 with code := ls).code` by rw[] >>
-  pop_assum SUBST1_TAC >>
-  (bc_next_FILTER_labels
-   |> SIMP_RULE std_ss [LET_THM]
-   |> Q.SPECL[`s1 with code := ls`,`s2 with code := ls`]
-   |> SIMP_RULE (srw_ss()) []
-   |> MP_CANON |> match_mp_tac ) >>
-  fs[])
 
 val bc_fetch_next_addr = store_thm("bc_fetch_next_addr",
   ``∀bc0 bs x bc.
@@ -1013,6 +718,7 @@ val Cenv_bs_imp_incsz = store_thm("Cenv_bs_imp_incsz",
 
 val bc_state_component_equality = DB.fetch"Bytecode""bc_state_component_equality"
 
+(*
 val compile_val = store_thm("compile_val",
   ``(∀c env exp res. Cevaluate c env exp res ⇒
       ∀v bc0 bc0c bc1 bs cs.
@@ -1334,6 +1040,7 @@ val repl_exp_val = store_thm("repl_exp_val",
   fs[] >>
   disch_then (qspecl_then [`bs.code`,`[]`,`bs0`,`cs`] mp_tac) >>
   rw[Abbr`bs0`]
+*)
 
 val with_same_pc = store_thm("with_same_pc",
   ``x with pc := x.pc = x``,
