compiler/bytecode/bytecodeTerminationScript.sml
@@ -6,6 +6,7 @@ val _ = export_rewrites["bc_fetch_aux_def"];
 val _ = save_thm("bc_fetch_def",bc_fetch_def);
 val _ = save_thm("bump_pc_def",bump_pc_def);
 val _ = save_thm("bc_find_loc_def",bc_find_loc_def);
+val _ = save_thm("bc_find_loc_aux_def",bc_find_loc_aux_def);
 val _ = save_thm("bc_next_rules",bc_next_rules);
 val _ = save_thm("bc_next_ind",bc_next_ind);
 val _ = save_thm("bc_next_cases",bc_next_cases);
