compiler/correctness/bytecodeExtraScript.sml
@@ -1,0 +1,38 @@
+open HolKernel bossLib boolLib boolSimps lcsymtacs
+open bytecodeTerminationTheory
+val _ = intLib.deprecate_int()
+val _ = new_theory"bytecodeExtra"
+
+val bc_fetch_with_stack = store_thm("bc_fetch_with_stack",
+  ``bc_fetch (s with stack := st) = bc_fetch s``,
+  rw[bc_fetch_def])
+
+val bump_pc_with_stack = store_thm("bump_pc_with_stack",
+  ``bump_pc (s with stack := st) = (bump_pc s) with stack := st``,
+  rw[bump_pc_def,bc_fetch_with_stack] >>
+  BasicProvers.EVERY_CASE_TAC)
+
+val bc_fetch_aux_MAP = store_thm("bc_fetch_aux_MAP",
+  ``!il f. (∀x. il (f x) = il x) ∧ (∀x. is_Label (f x) = is_Label x) ⇒
+      ∀ls n. (bc_fetch_aux (MAP f ls) il n = OPTION_MAP f (bc_fetch_aux ls il n))``,
+  ntac 2 gen_tac >> strip_tac >>
+  Induct >> rw[bc_fetch_aux_def])
+
+val bc_fetch_MAP = store_thm("bc_fetch_MAP",
+  ``∀f s. (∀x. s.inst_length (f x) = s.inst_length x) ∧ (∀x. is_Label (f x) = is_Label x) ⇒
+    (bc_fetch (s with <| code := MAP f s.code |>) = OPTION_MAP f (bc_fetch s))``,
+  rw[bc_fetch_def,bc_fetch_aux_MAP])
+
+val bc_find_loc_aux_NONE = store_thm("bc_find_loc_aux_NONE",
+  ``∀il l ls n. (bc_find_loc_aux ls il l n = NONE) ⇒ ¬MEM (Label l) ls``,
+  ntac 2 gen_tac >>
+  Induct >> rw[bc_find_loc_aux_def] >>
+  res_tac >> fs[])
+
+val bc_find_loc_aux_MEM = store_thm("bc_find_loc_aux_MEM",
+  ``∀il l ls n. (bc_find_loc_aux ls il l n ≠ NONE) ⇒ MEM (Label l) ls``,
+  ntac 2 gen_tac >>
+  Induct >> rw[bc_find_loc_aux_def] >>
+  res_tac)
+
+val _ = export_theory()
