compiler/correctness/compileLabelsScript.sml
@@ -1,0 +1,263 @@
+open HolKernel bossLib boolLib boolSimps listTheory rich_listTheory alistTheory finite_mapTheory lcsymtacs
+open miscTheory bytecodeTerminationTheory compileTerminationTheory bytecodeEvalTheory bytecodeExtraTheory
+val _ = intLib.deprecate_int()
+val _ = new_theory"compileLabels"
+
+val el_of_addr_def = Define`
+  (el_of_addr il n [] = NONE) ∧
+  (el_of_addr il n (x::xs) =
+   if is_Label x then OPTION_BIND (el_of_addr il n xs) (λm. SOME (m + 1)) else
+     if n = 0 then SOME (0:num) else
+       if n < il x + 1 then NONE else
+         OPTION_BIND (el_of_addr il (n - (il x + 1)) xs) (λm. SOME (m + 1)))`
+val _ = export_rewrites["el_of_addr_def"]
+
+val el_of_addr_LESS_LENGTH = store_thm("el_of_addr_LESS_LENGTH",
+  ``∀il ls n m. (el_of_addr il n ls = SOME m) ⇒ m < LENGTH ls``,
+  gen_tac >> Induct >> srw_tac[ARITH_ss][] >>
+  res_tac >> fsrw_tac[ARITH_ss][])
+
+val bc_fetch_aux_el_of_addr = store_thm("bc_fetch_aux_el_of_addr",
+  ``∀c il pc. bc_fetch_aux c il pc = OPTION_BIND (el_of_addr il pc c) (λn. SOME (EL n c))``,
+  Induct >> rw[] >>
+  Q.PAT_ABBREV_TAC`opt = el_of_addr il pcX c` >>
+  Cases_on `opt` >> fs[] >>
+  rw[GSYM arithmeticTheory.ADD1])
+
+val replace_lab_def = Define`
+  (replace_lab m (Jump (Lab l)) = Jump (Addr (FAPPLY m l))) ∧
+  (replace_lab m (JumpIf (Lab l)) = JumpIf (Addr (m ' l))) ∧
+  (replace_lab m (Call (Lab l)) = Call (Addr (m ' l))) ∧
+  (replace_lab m (PushPtr (Lab l)) = PushPtr (Addr (m ' l))) ∧
+  (replace_lab m i = i)`
+val _ = export_rewrites["replace_lab_def"]
+
+val is_Label_replace_lab = store_thm("is_Label_replace_lab",
+  ``∀x. is_Label (replace_lab m x) = is_Label x``,
+  Cases >> rw[] >> Cases_on `l` >> rw[])
+val _ = export_rewrites["is_Label_replace_lab"]
+
+val dest_Label_def = Define`(dest_Label (Label n) = n)`
+val _ = export_rewrites["dest_Label_def"]
+
+val good_il_def = Define`
+  good_il il =
+  (∀x. il (Jump x) = il (Jump ARB)) ∧
+  (∀x. il (JumpIf x) = il (JumpIf ARB)) ∧
+  (∀x. il (Call x) = il (Call ARB)) ∧
+  (∀x. il (PushPtr x) = il (PushPtr ARB))`
+
+val il_replace_lab = store_thm("il_replace_lab",
+  ``good_il il ⇒ ∀m x. (il (replace_lab m x) = il x)``,
+  rw[good_il_def] >>
+  Cases_on `x` >> rw[] >>
+  Cases_on `l` >> rw[])
+
+val calculate_labels_thm = store_thm("calculate_labels_thm",
+  ``∀il m n bc lbc m' n' bc'.
+      (calculate_labels il m n bc lbc = (m',n',bc')) ∧ ALL_DISTINCT (FILTER is_Label lbc) ⇒
+      (bc' = (REVERSE (FILTER ($~ o is_Label) lbc) ++ bc)) ∧
+      (let ls = MAP dest_Label (FILTER is_Label lbc) in
+        (m' = m |++ ZIP (ls, MAP (THE o combin$C (bc_find_loc_aux lbc il) n) ls))) ∧
+      (n' = n + SUM (MAP (SUC o il) (FILTER ($~ o is_Label) lbc)))``,
+  ho_match_mp_tac calculate_labels_ind >>
+  strip_tac >- (
+    rw[calculate_labels_def,LET_THM,FUPDATE_LIST_THM] ) >>
+  strip_tac >- (
+    rpt gen_tac >> strip_tac >>
+    simp_tac(std_ss)[Once calculate_labels_def] >>
+    rpt gen_tac >> strip_tac >>
+    `ALL_DISTINCT (FILTER is_Label lbc)` by (
+      pop_assum mp_tac >>
+      rpt (pop_assum kall_tac) >>
+      rw[] ) >>
+    res_tac >>
+    full_simp_tac(std_ss)[LET_THM] >>
+    rpt BasicProvers.VAR_EQ_TAC >>
+    pop_assum kall_tac >> pop_assum mp_tac >>
+    rpt (pop_assum kall_tac) >>
+    rw[FUPDATE_LIST_THM,bc_find_loc_aux_def] >>
+    AP_TERM_TAC >> AP_TERM_TAC >> AP_TERM_TAC >>
+    rw[MAP_EQ_f,MEM_MAP,MEM_FILTER] >>
+    AP_TERM_TAC >>
+    rw[bc_find_loc_aux_def] >>
+    fs[MEM_FILTER] >>
+    Cases_on `y` >> fs[]) >>
+  REPEAT (
+    strip_tac >- (
+      rpt gen_tac >> strip_tac >>
+      simp_tac(std_ss)[Once calculate_labels_def] >>
+      rpt gen_tac >> strip_tac >>
+      `ALL_DISTINCT (FILTER is_Label lbc)` by (
+        pop_assum mp_tac >>
+        rpt (pop_assum kall_tac) >>
+        rw[] ) >>
+      res_tac >>
+      full_simp_tac(std_ss)[LET_THM] >>
+      rpt BasicProvers.VAR_EQ_TAC >>
+      rpt (pop_assum kall_tac) >>
+      srw_tac[ARITH_ss][] >>
+      AP_TERM_TAC >> AP_TERM_TAC >> AP_TERM_TAC >>
+      rw[MAP_EQ_f,MEM_MAP,MEM_FILTER] >>
+      AP_TERM_TAC >>
+      rw[bc_find_loc_aux_def] )))
+
+val replace_labels_thm = store_thm("replace_labels_thm",
+  ``∀m a ls. (replace_labels m a ls = (REVERSE (MAP (replace_lab m) ls)) ++ a)``,
+  ho_match_mp_tac replace_labels_ind >> rw[replace_labels_def])
+
+val tac = (
+    rw[LET_THM] >>
+    match_mp_tac bc_eval1_SOME >>
+    Q.PAT_ABBREV_TAC`f = replace_lab X` >>
+    qspecl_then[`f`,`s1`] mp_tac bc_fetch_MAP >>
+    qunabbrev_tac`f` >> rw[il_replace_lab] >>
+    rw[bc_eval1_def] >>
+    fs[bc_eval_stack_thm] >>
+    fs[bump_pc_def] )
+
+val tac2 = (
+    rw[LET_THM] >>
+    match_mp_tac bc_eval1_SOME >>
+    Q.PAT_ABBREV_TAC`f = replace_lab X` >>
+    qspecl_then[`f`,`s1`] mp_tac bc_fetch_MAP >>
+    qunabbrev_tac`f` >>
+    Cases_on `l` >> rw[il_replace_lab] >>
+    srw_tac[DNF_ss][bc_eval1_def,LET_THM] >>
+    fs[bc_eval_stack_thm,bc_find_loc_def] >>
+    fs[FLOOKUP_DEF] >>
+    rw[bump_pc_with_stack] >>
+    rw[bump_pc_def] >>
+    fs[good_il_def] >>
+    metis_tac[optionTheory.SOME_11,optionTheory.NOT_SOME_NONE])
+
+val bc_next_MAP_replace_lab = store_thm("bc_next_MAP_replace_lab",
+  ``∀s1 s2. bc_next s1 s2 ⇒
+      ∀m. good_il s1.inst_length ∧
+      (∀l. FLOOKUP m l = bc_find_loc s1 (Lab l)) ⇒
+    let c = MAP (replace_lab m) s1.code in
+    bc_next (s1 with <| code := c |>) (s2 with <| code := c |>)``,
+  ho_match_mp_tac bc_next_ind >>
+  strip_tac >- tac >>
+  strip_tac >- tac2 >>
+  strip_tac >- tac2 >>
+  strip_tac >- tac2 >>
+  strip_tac >- tac >>
+  strip_tac >- tac >>
+  strip_tac >- tac2 >>
+  strip_tac >- tac >>
+  strip_tac >- tac >>
+  strip_tac >- tac >>
+  strip_tac >- tac >>
+  strip_tac >- tac )
+
+val bc_fetch_MEM = store_thm("bc_fetch_MEM",
+  ``(bc_fetch s1 = SOME i) ⇒ (MEM i s1.code)``,
+  rw[bc_fetch_def] >>
+  fs[bc_fetch_aux_el_of_addr] >>
+  rw[MEM_EL] >>
+  imp_res_tac el_of_addr_LESS_LENGTH >>
+  metis_tac[])
+
+val addrs_only_def = Define`
+  (addrs_only (Jump (Lab _)) = F) ∧
+  (addrs_only (JumpIf (Lab _)) = F) ∧
+  (addrs_only (Call (Lab _)) = F) ∧
+  (addrs_only (PushPtr (Lab _)) = F) ∧
+  (addrs_only _ = T)`
+val _ = export_rewrites["addrs_only_def"]
+
+val addrs_only_replace_lab = store_thm("addrs_only_replace_lab",
+  ``addrs_only (replace_lab m x)``,
+  Cases_on `x` >> rw[] >> Cases_on `l` >> rw[])
+val _ = export_rewrites["addrs_only_replace_lab"]
+
+val bc_fetch_aux_FILTER_labels = store_thm("bc_fetch_aux_FILTER_labels",
+  ``∀il ls n. bc_fetch_aux (FILTER ($~ o is_Label) ls) il n = bc_fetch_aux ls il n``,
+  gen_tac >> Induct >> rw[])
+val _ = export_rewrites["bc_fetch_aux_FILTER_labels"]
+
+val bc_fetch_FILTER_labels = store_thm("bc_fetch_FILTER_labels",
+  ``bc_fetch (s with code := FILTER ($~ o is_Label) s.code) = bc_fetch s``,
+  rw[bc_fetch_def])
+val _ = export_rewrites["bc_fetch_FILTER_labels"]
+
+val bc_next_FILTER_labels = store_thm("bc_next_FILTER_labels",
+  ``∀s1 s2. bc_next s1 s2 ⇒ EVERY addrs_only s1.code ⇒
+      let c = FILTER ($~ o is_Label) s1.code in
+      bc_next (s1 with <| code := c |>) (s2 with <| code := c |>)``,
+  ho_match_mp_tac bc_next_ind >>
+  rw[LET_THM] >>
+  rw[bc_eval1_thm] >>
+  srw_tac[DNF_ss][bc_eval1_def,LET_THM] >>
+  fs[bc_eval_stack_thm] >>
+  rw[bump_pc_def] >>
+  imp_res_tac bc_fetch_MEM >>
+  fs[EVERY_MEM] >>
+  res_tac >>
+  Cases_on `l` >> fs[bc_find_loc_def] >>
+  rw[bc_fetch_with_stack])
+
+val bc_next_compile_labels = store_thm("bc_next_compile_labels",
+  ``∀s1 s2. bc_next s1 s2 ⇒
+      (good_il s1.inst_length ∧
+       ALL_DISTINCT (FILTER is_Label s1.code)) ⇒
+      let c = compile_labels s1.inst_length s1.code in
+      bc_next (s1 with <| code := c |>) (s2 with <| code := c |>)``,
+  rw[compile_labels_def,replace_labels_thm] >>
+  imp_res_tac calculate_labels_thm >>
+  rpt BasicProvers.VAR_EQ_TAC >>
+  qunabbrev_tac`c` >>
+  rw[MAP_REVERSE] >>
+  `∀x. ($~ o is_Label) (replace_lab m x) = ($~ o is_Label) x` by rw[] >>
+  rw[MAP_FILTER] >>
+  qmatch_abbrev_tac `bc_next (s1 with code := FILTER P ls) (s2 with code := FILTER P ls)` >>
+  `EVERY addrs_only ls` by (
+    qunabbrev_tac`ls` >>
+    rw[EVERY_MAP] ) >>
+  `bc_next (s1 with code := ls) (s2 with code := ls)` by (
+    qunabbrev_tac`ls` >>
+    match_mp_tac (MP_CANON(SIMP_RULE(srw_ss())[LET_THM]bc_next_MAP_replace_lab)) >>
+    rw[bc_find_loc_def] >>
+    fs[LET_THM] >>
+    qmatch_abbrev_tac `FLOOKUP (fm |++ ls) l = X` >>
+    Cases_on `X` >- (
+      `ALOOKUP (REVERSE ls) l = NONE` by (
+        qunabbrev_tac`ls` >>
+        rw[ALOOKUP_FAILS,ZIP_MAP] >>
+        rw[MAP_MAP_o,combinTheory.o_DEF] >>
+        `¬MEM (Label l) s1.code` by metis_tac[bc_find_loc_aux_NONE] >>
+        `¬MEM (Label l) (FILTER is_Label s1.code)` by rw[MEM_FILTER] >>
+        rw[MEM_MAP] >>
+        Cases_on `x` >> rw[MEM_FILTER] >>
+        PROVE_TAC[] ) >>
+      imp_res_tac FLOOKUP_FUPDATE_LIST_ALOOKUP_NONE >>
+      fs[Abbr`fm`] ) >>
+    `ALOOKUP (REVERSE ls) l = SOME x` by (
+      match_mp_tac ALOOKUP_ALL_DISTINCT_MEM >>
+      qunabbrev_tac`ls` >>
+      rw[REVERSE_ZIP,MAP_ZIP,ALL_DISTINCT_REVERSE] >- (
+        match_mp_tac ALL_DISTINCT_MAP_INJ >> fs[] >>
+        qx_gen_tac `a` >> qx_gen_tac `b` >>
+        Cases_on `a` >> Cases_on `b` >> rw[MEM_FILTER] ) >>
+      `MEM (Label l) s1.code` by
+        metis_tac[bc_find_loc_aux_MEM,optionTheory.NOT_SOME_NONE] >>
+      `MEM (Label l) (FILTER is_Label s1.code)` by rw[MEM_FILTER] >>
+      pop_assum (strip_assume_tac o SIMP_RULE (srw_ss()) [MEM_EL]) >>
+      rw[MEM_ZIP] >>
+      qexists_tac `n` >>
+      pop_assum (assume_tac o SYM) >>
+      rw[EL_MAP] ) >>
+    imp_res_tac FLOOKUP_FUPDATE_LIST_ALOOKUP_SOME >>
+    fs[] ) >>
+  qunabbrev_tac`P` >>
+  `ls = (s1 with code := ls).code` by rw[] >>
+  pop_assum SUBST1_TAC >>
+  (bc_next_FILTER_labels
+   |> SIMP_RULE std_ss [LET_THM]
+   |> Q.SPECL[`s1 with code := ls`,`s2 with code := ls`]
+   |> SIMP_RULE (srw_ss()) []
+   |> MP_CANON |> match_mp_tac ) >>
+  fs[])
+
+val _ = export_theory()
